SocketIO proposal

test/artifact/pneutube/PaddedFileIO.fst
@@ -8,9 +8,28 @@ open Hacl.UInt64
 
 open FileIO.Types
 
+module U32 = FStar.UInt32
+module H32 =  Hacl.UInt32
 module U64 = FStar.UInt64
 module H64 =  Hacl.UInt64
 module B   = FStar.Buffer
+
+#reset-options "--initial_fuel 0 --max_fuel 0"
+private val lemma_max_uint8: n:nat -> Lemma
+ (requires (n = 8))
+ (ensures  (pow2 n = 256))
+ [SMTPat (pow2 n)]
+let lemma_max_uint8 n = assert_norm(pow2 8 = 256)
+private val lemma_max_uint32: n:nat -> Lemma
+ (requires (n = 32))
+ (ensures  (pow2 n = 4294967296))
+ [SMTPat (pow2 n)]
+let lemma_max_uint32 n = assert_norm(pow2 32 = 4294967296)
+private val lemma_max_uint64: n:nat -> Lemma
+ (requires (n = 64))
+ (ensures  (pow2 n = 18446744073709551616))
+ [SMTPat (pow2 n)]
+let lemma_max_uint64 n = assert_norm(pow2 64 = 18446744073709551616)
 
 (* Need to get rid of these  following ones *)
 type string = seq u8
@@ -19,84 +38,160 @@ inline_for_extraction val zero: u64
 inline_for_extraction let zero = 0uL
 (* The above need to come from some library module *)
 
+type bufsize = x:U64.t{U64.v x < pow2 32}
+
+private let bufsize_bound (x:bufsize) : Lemma (requires (True)) (ensures (U32.v (Int.Cast.uint64_to_uint32 x) = U64.v x)) [SMTPat (Int.Cast.uint64_to_uint32 x)] = Math.Lemmas.modulo_lemma (U64.v x) (pow2 32)
 
 (* File System Buffer Size, currently 256KB *)
 inline_for_extraction val max_block_size: u64
 inline_for_extraction let max_block_size = 262144uL
 
+
 assume val file_state: FStar.HyperStack.mem -> file_handle -> GTot fd_state
 assume val file_offset: FStar.HyperStack.mem -> file_handle -> GTot u64
 assume val file_buffer: FStar.HyperStack.mem -> file_stat -> GTot (buffer h8)
-assume val file_content: FStar.HyperStack.mem -> file_stat -> GTot (seq h8)
 
-let file_sub (m:FStar.HyperStack.mem) (f:file_handle) (i:u64) (j:u64) =	
+let file_sub (m:FStar.HyperStack.mem) (f:file_handle) (i:u64) (j:u64{U64.v j + U64.v i <= length (file_buffer m f.stat)}) =
     B.sub (file_buffer m f.stat) (Int.Cast.uint64_to_uint32 i) (Int.Cast.uint64_to_uint32 j)
-    
+
+
+(* A live file handle maps to a buffer which max_length is the size indicated in the file_stat *)
+let live_fh h (fh:file_handle) : GTot Type0 =
+  live h (file_buffer h fh.stat)
+  /\ max_length (file_buffer h fh.stat) = H64.v fh.stat.size
+  /\ length (file_buffer h fh.stat) = H64.v fh.stat.size
+  /\ U64.v (file_offset h fh) <= H64.v fh.stat.size
+
+(* Type of a workable file *)
+let live_file h (f:buffer file_handle) : GTot Type0 =
+  length f = 1 /\ live h f /\ (let fh = get h f 0 in live_fh h fh)
+
+(* Files are not changed through reads/writes *)
+let same_file h f h' f' : GTot Type0 =
+  live_file h f /\ live_file h' f'
+  /\ (let fh = get h f 0 in let fh' = get h' f' 0 in  fh.stat == fh'.stat)
+
+val file_content: h:FStar.HyperStack.mem -> fs:file_stat{live h (file_buffer h fs)}  -> GTot (seq h8)
+let file_content m fs = as_seq m (file_buffer m fs)
+
 
 (* TODO: check the live/modifies clauses below *)
-assume val file_open_read_sequential: n:uint8_p -> fb:buffer file_handle -> Stack fresult
-    (requires (fun h -> length fb = 1 /\ live h fb))
-    (ensures  (fun h0 s h1 -> match s with 
-	      	       	    | FileOk -> 
-			      live h1 fb /\
+assume val file_open_read_sequential: n:uint8_p ->
+  fb:buffer file_handle{disjoint n fb /\ length fb = 1} ->
+  Stack fresult
+    (requires (fun h -> live h fb /\ live h n))
+    (ensures  (fun h0 s h1 -> (match s with
+	      	       	    | FileOk ->
 			      modifies_1 fb h0 h1 /\
+                              live_file h1 fb /\
 			      (let fh = get h1 fb 0 in
-    	      	     	       file_state h1 fh = FileOpen /\	
-			       file_offset h1 fh = zero /\	
-			       file_content h0 fh.stat = file_content h1 fh.stat)
-			    | _ -> true))
-
-
-assume val file_open_write_sequential: file_stat -> fb:buffer file_handle -> Stack fresult
-    (requires (fun h -> length fb = 1 /\ live h fb))
-    (ensures  (fun h0 s h1 -> match s with 
-    	      	      	    | FileOk -> 
-			      live h1 fb /\
-			      (let fh = get h1 fb 0 in
-    	      	      	       file_state h1 fh = FileOpen /\ 
+    	      	     	       file_state h1 fh = FileOpen /\
 			       file_offset h1 fh = zero /\
-			       file_content h0 fh.stat = file_content h1 fh.stat)
+			       length (file_buffer h1 fh.stat) = max_length (file_buffer h1 fh.stat))
+			       (* /\ file_content h0 fh.stat == file_content h1 fh.stat) *)
+			    | _ -> true)))
+
+
+assume val file_open_write_sequential: file_stat ->
+  fb:buffer file_handle{length fb = 1} ->
+  Stack fresult
+    (requires (fun h -> live h fb))
+    (ensures  (fun h0 s h1 -> match s with
+    	      	      	    | FileOk ->
+			      live_file h1 fb /\
+			      (let fh = get h1 fb 0 in
+    	      	      	       file_state h1 fh = FileOpen /\
+			       file_offset h1 fh = zero /\
+			       length (file_buffer h1 fh.stat) = max_length (file_buffer h1 fh.stat))
+			       (* file_content h0 fh.stat == file_content h1 fh.stat) *)
 			    | _ -> true))
 
-assume val file_next_read_buffer: fb:buffer file_handle -> len:u64 -> Stack uint8_p
-    (requires (fun h0 -> U64.v len <= U64.v max_block_size /\
-    	      	         length fb = 1 /\ live h0 fb /\
-    	      	         (let f = get h0 fb 0 in
-			  file_state h0 f = FileOpen)))
-    (ensures  (fun h0 s h1 -> let f = get h1 fb 0 in
-    	      	              let i = file_offset h0 f in
-    	      	      	      let j = U64 (file_offset h0 f +^ len) in
-			      modifies_1 s h0 h1 /\
-    	      	      	      file_state h1 f = FileOpen /\ 
-    	      	      	      file_offset h1 f = j /\
-			      file_content h0 f.stat = file_content h1 f.stat /\
-			      ((U64.v i <= H64.v f.stat.size /\ U64.v j <= H64.v f.stat.size) ==> s = file_sub h1 f i len)(*  /\ *)
-			      (* ((U64.v i <= v f.stat.size /\ U64.v j > v f.stat.size) ==>  B.sub s 0ul (Int.Cast.uint64_to_uint32 ((f.stat.size -^ i))) = file_sub h1 f i (f.stat.size -^ i)) *)
-                              ))
-			      
+private let sint64_to_uint64 (x:H64.t) : GTot U64.t = U64.uint_to_t (H64.v x)
+private let sint64_to_uint32 (x:H64.t) : GTot U32.t = Int.Cast.uint64_to_uint32 (U64.uint_to_t (H64.v x))
 
-assume val file_next_write_buffer: fb:buffer file_handle -> len:u64 -> Stack uint8_p
-    (requires (fun h0 -> U64.v len <= U64.v max_block_size /\
-    	      	         length fb = 1 /\ live h0 fb /\
-    	      	         (let f = get h0 fb 0 in
-			  file_state h0 f = FileOpen)))
-    (ensures  (fun h0 s h1 -> let f = get h1 fb 0 in
-    	      	              let i = file_offset h0 f in
-    	      	      	      let j = U64 (file_offset h0 f +^ len) in
-			      modifies_1 s h0 h1 /\
-    	      	      	      file_state h1 f = FileOpen /\ 
-    	      	      	      file_offset h1 f = j /\
-			      file_content h0 f.stat = file_content h1 f.stat /\
-			      ((U64.v i <= v f.stat.size /\ U64.v j <= v f.stat.size) ==> s = file_sub h1 f i len)(*  /\ *)
-			      (* ((U64.v i <= v f.stat.size /\ U64.v j > v f.stat.size) ==>  sub s zero (f.stat.size -^ i) = file_sub h1 f i (f.stat.size -^ i)) *)
-                              ))
-			      
 
-assume val file_close: fb:buffer file_handle -> Stack bool
-    (requires (fun h0 -> length fb = 1 /\ live h0 fb /\
+(* assume val file_next_read_buffer: fb:buffer file_handle{length fb = 1} -> *)
+(*   len:u64 -> *)
+(*   Stack uint8_p *)
+(*     (requires (fun h0 -> U64.v len <= U64.v max_block_size /\ *)
+(*     	      	         length fb = 1 /\ live h0 fb /\ *)
+(*     	      	         (let f = get h0 fb 0 in *)
+(* 			  file_state h0 f = FileOpen))) *)
+(*     (ensures  (fun h0 s h1 -> live h1 fb /\ let f = get h1 fb 0 in *)
+(*     	      	              let i = (file_offset h0 f) in *)
+(*     	      	      	      let j = Hacl.Cast.uint64_to_sint64 (U64 (file_offset h0 f +^ len)) in *)
+(* 			      modifies_1 s h0 h1 /\ *)
+(*     	      	      	      file_state h1 f = FileOpen /\ *)
+(*     	      	      	      Hacl.Cast.uint64_to_sint64 (file_offset h1 f) == j /\ *)
+(* 			      file_content h0 f.stat == file_content h1 f.stat /\ *)
+(* 			      ((U64.v i <= H64.v f.stat.size /\ H64.v j <= H64.v f.stat.size) ==> s == file_sub h1 f i len) /\ *)
+(* 			      ((U64.v i <= v f.stat.size /\ H64.v j > v f.stat.size) ==> (B.sub s 0ul (sint64_to_uint32 ((f.stat.size -^ Hacl.Cast.uint64_to_sint64 i))) == file_sub h1 f i (sint64_to_uint64 (f.stat.size -^ Hacl.Cast.uint64_to_sint64 i)))) *)
+(*                               )) *)
+
+let file_next_read_buffer_pre h (fb:buffer file_handle{length fb = 1}) (len:U64.t) : GTot Type0 =
+  live_file h fb /\ U64.v len <= U64.v max_block_size
+  /\ (let fh = get h fb 0 in file_state h fh = FileOpen
+    /\ U64.v (file_offset h fh) + U64.v len <= H64.v fh.stat.size)
+
+let file_next_read_buffer_post h0 (s:uint8_p) h1 (fb:buffer file_handle{length fb = 1})
+                               (len:bufsize) : GTot Type0 =
+  file_next_read_buffer_pre h0 fb len
+  /\ live_file h0 fb /\ live_file h1 fb /\ same_file h0 fb h1 fb
+  /\ (let fh0 = get h0 fb 0 in let fh1 = get h1 fb 0 in
+      U64.v (file_offset h1 fh1) = U64.v (file_offset h0 fh0) + U64.v len
+      /\ file_state h1 fh1 = FileOpen
+      /\ s == Buffer.sub (file_buffer h0 fh0.stat) (Int.Cast.uint64_to_uint32 (file_offset h0 fh0)) (Int.Cast.uint64_to_uint32 len))
+  /\ modifies_0 h0 h1
+
+
+assume val file_next_read_buffer:
+  fb:buffer file_handle{length fb = 1} ->
+  len:bufsize ->
+  Stack uint8_p
+    (requires (fun h0 -> file_next_read_buffer_pre h0 fb len))
+    (ensures  (fun h0 s h1 -> file_next_read_buffer_post h0 s h1 fb len))
+
+
+let file_next_write_buffer_pre h (fb:buffer file_handle{length fb = 1}) (len:U64.t) : GTot Type0 =
+  live_file h fb /\ U64.v len <= U64.v max_block_size
+  /\ (let fh = get h fb 0 in file_state h fh = FileOpen
+    /\ U64.v (file_offset h fh) + U64.v len <= H64.v fh.stat.size)
+
+let file_next_write_buffer_post h0 (s:uint8_p) h1 (fb:buffer file_handle{length fb = 1})
+                               (len:bufsize) : GTot Type0 =
+  file_next_read_buffer_pre h0 fb len
+  /\ live_file h0 fb /\ live_file h1 fb /\ same_file h0 fb h1 fb
+  /\ (let fh0 = get h0 fb 0 in let fh1 = get h1 fb 0 in
+      U64.v (file_offset h1 fh1) = U64.v (file_offset h0 fh0) + U64.v len
+      /\ file_state h1 fh1 = FileOpen
+      /\ s == Buffer.sub (file_buffer h0 fh0.stat) (Int.Cast.uint64_to_uint32 (file_offset h0 fh0)) (Int.Cast.uint64_to_uint32 len))
+  /\ modifies_0 h0 h1
+
+assume val file_next_write_buffer: fb:buffer file_handle{length fb = 1} -> len:bufsize -> Stack uint8_p
+    (requires (fun h0 -> file_next_write_buffer_pre h0 fb len))
+    (ensures  (fun h0 s h1 -> file_next_read_buffer_post h0 s h1 fb len))
+
+(* assume val file_next_write_buffer: fb:buffer file_handle -> len:u64 -> Stack uint8_p *)
+(*     (requires (fun h0 -> U64.v len <= U64.v max_block_size /\ *)
+(*     	      	         length fb = 1 /\ live h0 fb /\ *)
+(*     	      	         (let f = get h0 fb 0 in *)
+(* 			  file_state h0 f = FileOpen))) *)
+(*     (ensures  (fun h0 s h1 -> let f = get h1 fb 0 in *)
+(*     	      	              let i = file_offset h0 f in *)
+(*     	      	      	      let j = U64 (file_offset h0 f +^ len) in *)
+(* 			      modifies_1 s h0 h1 /\ *)
+(*     	      	      	      file_state h1 f = FileOpen /\ *)
+(*     	      	      	      file_offset h1 f = j /\ *)
+(* 			      file_content h0 f.stat = file_content h1 f.stat /\ *)
+(* 			      ((U64.v i <= v f.stat.size /\ U64.v j <= v f.stat.size) ==> s = file_sub h1 f i len)(\*  /\ *\) *)
+(* 			      (\* ((U64.v i <= v f.stat.size /\ U64.v j > v f.stat.size) ==>  sub s zero (f.stat.size -^ i) = file_sub h1 f i (f.stat.size -^ i)) *\) *)
+(*                               )) *)
+
+
+assume val file_close: fb:buffer file_handle{length fb = 1} -> Stack bool
+    (requires (fun h0 -> length fb = 1 /\ live_file h0 fb /\
                          (let f = get h0 fb 0 in
 			  file_state h0 f = FileOpen)))
-    (ensures  (fun h0 r h1 -> r ==> 
-                         (let f = get h1 fb 0 in
-       	      	      	  file_state h1 f = FileClosed /\
-    			  file_content h0 f.stat = file_content h1 f.stat)))
+    (ensures  (fun h0 r h1 -> live_file h0 fb /\ live_file h1 fb /\ same_file h0 fb h1 fb
+      /\ (r ==> (let f = get h1 fb 0 in file_state h1 f = FileClosed /\
+    			              file_content h0 f.stat == file_content h1 f.stat))))
